More easily moved theorems from CakeML (this time to finite_map)

src/finite_map/finite_mapScript.sml
@@ -623,6 +623,10 @@ val SUBMAP_FUPDATE_EQN = Q.store_thm(
   METIS_TAC []);
 val _ = export_rewrites ["SUBMAP_FUPDATE_EQN"]
 
+Theorem SUBMAP_FDOM_SUBSET
+  `f1 SUBMAP f2 ==> FDOM f1 SUBSET FDOM f2`
+  (srw_tac[][SUBMAP_DEF,SUBSET_DEF]);
+
 (*---------------------------------------------------------------------------
     Restriction
  ---------------------------------------------------------------------------*)
@@ -993,6 +997,10 @@ val FLOOKUP_SUBMAP = store_thm(
   "FLOOKUP_SUBMAP",
   ``f SUBMAP g /\ (FLOOKUP f k = SOME v) ==> (FLOOKUP g k = SOME v)``,
   SRW_TAC [][FLOOKUP_DEF, SUBMAP_DEF] THEN METIS_TAC []);
+
+Theorem SUBMAP_FLOOKUP_EQN
+  `f SUBMAP g <=> !x y. (FLOOKUP f x = SOME y) ==> (FLOOKUP g x = SOME y)`
+  (rw[SUBMAP_DEF,FLOOKUP_DEF] \\ METIS_TAC[]);
 
 val SUBMAP_FUPDATE_FLOOKUP = store_thm(
   "SUBMAP_FUPDATE_FLOOKUP",
@@ -1636,6 +1644,13 @@ val FAPPLY_FUPD_EQ = prove(
 
 
 (* (pseudo) injectivity results about fupdate *)
+Theorem FEMPTY_FUPDATE_EQ
+  `!x y. (FEMPTY |+ x = FEMPTY |+ y) <=> (x = y)`
+  (Cases >> Cases >> srw_tac[][fmap_eq_flookup,FDOM_FUPDATE,FLOOKUP_UPDATE] >>
+  Cases_on`q=q'`>>srw_tac[][] >- (
+    srw_tac[][EQ_IMP_THM] >>
+    pop_assum(qspec_then`q`mp_tac) >> srw_tac[][] ) >>
+  qexists_tac`q`>>srw_tac[][])
 
 val FUPD11_SAME_KEY_AND_BASE = store_thm(
   "FUPD11_SAME_KEY_AND_BASE",
@@ -1693,6 +1708,11 @@ val FDOM_FUPDATE_LIST = store_thm(
   ASM_SIMP_TAC (srw_ss()) [FUPDATE_LIST_THM,
                            FDOM_FUPDATE, pairTheory.FORALL_PROD,
                            EXTENSION] THEN PROVE_TAC []);
+
+Theorem FUPDATE_LIST_EQ_FEMPTY
+  `!fm ls. (fm |++ ls = FEMPTY) <=> (fm = FEMPTY) /\ (ls = [])`
+  (srw_tac[][EQ_IMP_THM,FUPDATE_LIST_THM] >>
+  full_simp_tac(srw_ss())[GSYM fmap_EQ_THM,FDOM_FUPDATE_LIST])
 
 val FUPDATE_LIST_SAME_UPDATE = store_thm(
   "FUPDATE_LIST_SAME_UPDATE",
@@ -2753,6 +2773,37 @@ val FUPDATE_LIST_ALL_DISTINCT_PERM = store_thm("FUPDATE_LIST_ALL_DISTINCT_PERM",
 
 end
 (* end CakeML lemmas *)
+
+(* ----------------------------------------------------------------------
+    FDIFF
+
+    Removes a whole bunch of keys at once
+   ---------------------------------------------------------------------- *)
+
+val FDIFF_def = Define `FDIFF f1 s = DRESTRICT f1 (COMPL s)`;
+
+Theorem FDOM_FDIFF[simp]
+  `x IN FDOM (FDIFF refs f2) <=> x IN FDOM refs /\ x NOTIN f2`
+  (full_simp_tac(srw_ss())[FDIFF_def,DRESTRICT_DEF]);
+
+val NUM_NOT_IN_FDOM =
+  MATCH_MP IN_INFINITE_NOT_FINITE (CONJ INFINITE_NUM_UNIV
+    (Q.ISPEC `f:num|->'a` FDOM_FINITE))
+  |> SIMP_RULE std_ss [IN_UNIV]
+  |> curry save_thm "NUM_NOT_IN_FDOM";
+
+val EXISTS_NOT_IN_FDOM_LEMMA = Q.prove(
+  `?x. ~(x IN FDOM (refs:num|->'a))`,
+  METIS_TAC [NUM_NOT_IN_FDOM]);
+
+Theorem LEAST_NOTIN_FDOM
+  `(LEAST ptr. ptr NOTIN FDOM (refs:num|->'a)) NOTIN FDOM refs`
+  (ASSUME_TAC
+     (EXISTS_NOT_IN_FDOM_LEMMA |> SIMP_RULE std_ss [whileTheory.LEAST_EXISTS])>>
+   fs[]);
+
+
+
 
 (*---------------------------------------------------------------------------*)
 (* Add fmap type to the TypeBase. Notice that we treat keys as being of size *)
